src/michael/path.lean
@@ -1,59 +1,174 @@
+-- authorship note: we pulled things from mathlib:hedetniemi without looking carefully at authorship.
+-- we'll have to backsolve for the author list later
 import michael.simple_graph
+import tactic.omega
+import tactic.apply_fun
 
 universes u
 variables {V : Type u}
 
+section list
+#check list.nth_le_zero 
+
+@[simp] lemma list.cons_nth_le_succ
+  {α : Type*} {hd : α} (tl : list α) 
+  (n : ℕ) (hn : n + 1 < (tl.cons hd).length) :
+(tl.cons hd).nth_le (n + 1) hn = tl.nth_le n (by tidy) := rfl
+
+lemma list.tail_nth_le
+  {α : Type*} (l : list α) 
+  (n : ℕ) (hn : n < l.tail.length) :
+l.tail.nth_le n hn = l.nth_le (n + 1) (by { simp at hn, omega, }) := 
+by { cases l, tidy }
+
+
+end list
+
 namespace simple_graph
 variables (G : simple_graph V)
 
--- TODO: this could literally be implemented with a list and a pairwise adjacent constraint. 
--- Then we'd have more lemmas available and `mem_cons` would be ~just an application of of the same for lists. 
-/-- A path is an ordered list of vertices where consecutive elements are adjacent. -/
-inductive path : V → V → Type u
-| nil  : Π (v : V), path v v 
-| cons : Π {v s t : V} (e : G.E) (hv : v ∈ e) (hs : s ∈ e) (l : path s t), path v t
+/-- Morally, a path is an alternating list of vertices and edges, 
+  with incidences between adjacent objects -/
+@[ext] structure path :=
+(head : V)
+(tail : list V)
+(edges : list G.E)
+(length_eq : edges.length = tail.length)
+(adj : ∀ (n : ℕ) (hn : n < edges.length), 
+  (list.cons head tail).nth_le n (by { simp; omega }) ∈ edges.nth_le n hn ∧ 
+  (list.cons head tail).nth_le (n + 1) (by { simp; omega }) ∈ edges.nth_le n hn)
 
--- notation a :: b := path.cons a b
+
 namespace path
-variables {G}
-/-- For e an edge and p a path, G.mem e p is true if the edge lies on the path. -/
-inductive mem : Π {s t : V} (e : G.E) (p : G.path s t), Prop
-| nil : ∀ {v} (e : G.E) (h : false), mem e (path.nil v)
-| head : ∀ {v s t : V} (e : G.E) (hv : v ∈ e) (hs : s ∈ e) (tl : G.path v t), mem e (tl.cons e hs hv)
-| tail : ∀ {v s t : V} (e e' : G.E) (hv : v ∈ e) (hs : s ∈ e) (tl : G.path v t) (h : mem e' tl) , mem e' (tl.cons e hs hv)
+variables {G} 
+variables (p : G.path)
 
-instance has_mem_edge {s t : V} : has_mem G.E (G.path s t) := 
-{ mem := mem }
+/-- The ordered list of all vertices in p, starting at p.head. -/
+def vertices : list V := p.head :: p.tail 
 
-/-- For e an edge and p a path, G.mem e p is true if the edge lies on the path. -/
-inductive vmem : Π {s t : V} (v : V) (p : G.path s t), Prop
-| nil : ∀ v, vmem v (path.nil v)
-| head : ∀ {v s t : V} (p : G.path s t), vmem s p
-| tail : ∀ {v s t : V} (e : G.E) (hv : v ∈ e) (hs : s ∈ e) (tl : G.path v t) (h : vmem v tl), vmem v (tl.cons e hs hv)
+/-- The number of edges in p. -/
+def length : ℕ := p.tail.length
 
-instance has_mem_vertex {s t : V} : has_mem V (G.path s t) := 
-{ mem := vmem }
+@[simp] lemma tail_length_eq : p.tail.length = p.length := rfl
+@[simp] lemma edges_length_eq : p.edges.length = p.length :=  by simp [p.length_eq]
 
-inductive is_trail : Π {s t} (p : G.path s t), Prop
-| nil : ∀ v, is_trail (path.nil v)
-| tail : ∀ {v s t} (e : G.E) (hv : v ∈ e) (hs : s ∈ e) (tl : G.path v t) (h : ¬ tl.mem e), is_trail (tl.cons e hs hv)
+-- variables {s t : V}
 
-def is_Eulerian {x y} (p : G.path x y) : Prop :=
-p.is_trail ∧ ∀ e, p.mem e
+variables {p}
+/-- p.edge_mem e holds if e is an edge along path p. -/
+def edge_mem (e : G.E) (p : G.path) : Prop := e ∈ p.edges
+-- this instance doesn't fire and I don't know why
+instance has_mem_edge : has_mem G.E G.path := 
+{ mem := edge_mem }
 
-lemma no_edge_in_nil {d x y : V} (e : G.E) : ¬ (path.nil d).mem e :=
-by rintro ⟨⟩
+/-- p.vertex_mem v holds if v is a vertex along path p. -/
+def vertex_mem (v : V) (p : G.path) : Prop := v ∈ p.vertices
+instance has_mem_vertices : has_mem V G.path := 
+{ mem := vertex_mem }
+variables (p)
 
-lemma path.mem_cons
- {v s t : V} (e hd : G.E) (hv : v ∈ e) (hs : s ∈ e) (tl : G.path v t) :
- (path.cons e hs hv tl).mem e ↔ e = hd ∨ tl.mem e :=
+/-- The empty path based at vertex v. -/
+def empty (v : V) : G.path :=
+{ head := v,
+  tail := list.nil,
+  edges := list.nil,
+  length_eq := rfl,
+  adj := by rintros _ ⟨_⟩ }
+
+instance [inhabited V] : inhabited G.path := { default := empty (arbitrary V) }
+
+lemma edge_mem_empty {v : V} (e : G.E) : ¬ (empty v).edge_mem e :=
+by simp [empty, edge_mem]
+
+lemma vertex_mem_empty {u v : V} : u ∈ (@empty _ G v) ↔ u = v :=
+by { unfold has_mem.mem vertex_mem, simp [empty, vertices], apply or_false }
+
+/-- p.cons e hp hs is the path extending `p` by edge `e`. -/
+def cons {s : V} (e : G.E) (hp : p.head ∈ e) (hs : s ∈ e) : G.path :=
+{ head := s,
+  tail := p.vertices,
+  edges := list.cons e p.edges,
+  length_eq := by { simp [vertices] },
+  adj := begin
+    intros n hn, simp only [list.length] at hn,
+    cases n, { simp, tauto },
+    simp; apply p.adj,
+  end }
+
+@[simp] lemma edge_mem_cons {s : V} (hd e : G.E) (hp : p.head ∈ hd) (hs : s ∈ hd) : 
+  (p.cons hd hp hs).edge_mem e ↔ e = hd ∨ p.edge_mem e :=
+by simp [path.cons, path.vertices, edge_mem]
+
+@[simp] lemma vertex_mem_cons {v s : V} (hd : G.E) (hp : p.head ∈ hd) (hs : s ∈ hd) : 
+  v ∈ (p.cons hd hp hs) ↔ v = s ∨ v ∈ p :=
+by refl
+
+@[simp] lemma cons_length {v : V} (e : G.E) (hs : p.head ∈ e) (hv : v ∈ e) : 
+  (p.cons e hs hv).length = p.length + 1 :=
+by { unfold cons length, simp [vertices] }
+
+lemma edges_eq_nil_iff : p.edges = list.nil ↔ p.tail = list.nil :=
+by rw [← list.length_eq_zero, p.length_eq, list.length_eq_zero]
+
+lemma length_eq_zero_iff_eq_empty : p.length = 0 ↔ p = empty p.head :=
 begin
-  by_cases h : e = hd, { simp [h, mem.head] },
-  split, intro a, 
-  cases a,
-  sorry,
-  sorry,
+  erw list.length_eq_zero,
+  split; intro h, swap, rw h, simp [empty],
+  ext, work_on_goal 2 {rw ← edges_eq_nil_iff at h},
+  any_goals {simp [empty, h]},
 end
 
+lemma cases_on' [nonempty V] : 
+  (∃ v, p = empty v) ∨
+  ∃ (tl : G.path) v e (hs : tl.head ∈ e) (hv : v ∈ e) , p = tl.cons e hs hv :=
+begin
+  inhabit V,
+  cases hp : p.edges with hd tl, 
+  { left, use p.head, ext, { simp [empty] }, 
+    { suffices : p.tail = list.nil, { simp [empty, this] },
+      rwa edges_eq_nil_iff at hp },
+    simp [hp, empty] }, 
+  have hp_nil : ¬ p.edges = list.nil, { simp [hp] },
+  rw edges_eq_nil_iff at hp_nil,
+
+  cases p.adj 0 _ with hv hs, simp only [list.nth_le, zero_add] at hs, 
+  repeat { rw list.nth_le_zero at * }, 
+  set q : G.path := { head := p.tail.head,
+    tail := list.tail p.tail,
+    edges := list.tail p.edges,
+    length_eq := by simp [p.length_eq],
+    adj := _},
+  swap, { intros, have := p.adj (n + 1) (by {simp only [list.length_tail] at hn, omega}), 
+    simp only [list.nth_le] at this ⊢, 
+    iterate 2 { rw list.tail_nth_le }, 
+    convert this, apply list.cons_head_tail hp_nil },
+  right, use [q, p.head, hd], 
+  simp only [hp, list.head] at hs hv, swap, { simp [hp] },
+  dsimp, use [hs, hv], 
+  ext, 
+  { simp [path.cons] },
+  { dsimp [q, path.cons, path.vertices], rwa list.cons_head_tail, },
+  { dsimp [q, path.cons], simp [hp] },
+end
+
+lemma induction_on [nonempty V] 
+  (P : G.path → Prop)
+  (P_empty : ∀ v, P $ empty v) 
+  (P_inductive : ∀ p e hs {v} (hv : v ∈ e), P p → P (p.cons e hs hv)) : 
+P p :=
+begin
+  suffices : ∀ k (q : G.path), q.length = k → P q, { apply this p.length, refl },
+  intro k, induction k with k hk, { intros, convert P_empty _, rwa ← length_eq_zero_iff_eq_empty },
+  intro q, rcases q.cases_on' with ⟨_,rfl⟩|⟨_,_,_,_,_,rfl⟩, { intro, apply P_empty },
+  intro, apply P_inductive, apply hk, simp at a, omega,
+end
+
+/-- p.is_trail if p has no repeated edges. -/
+def is_trail : Prop := list.nodup p.edges
+
+/-- p.is_Eulerian if p hits each edge exactly once. -/
+def is_Eulerian : Prop := ∀ e : G.E, p.edge_mem e
+
 end path
+
 end simple_graph
